WeirdLogic/Example2.lean
@@ -1,0 +1,118 @@
+import Mathlib.Computability.ContextFreeGrammar
+
+import Lgtm.Hyper.ProofMode
+import Lgtm.Hyper.ArraysFun
+import Lgtm.Unary.Lang
+import Lgtm.Experiments.HyperCommon
+
+import WeirdLogic.Gram
+import WeirdLogic.WLogic
+import WeirdLogic.WTriple
+import WeirdLogic.Util
+import WeirdLogic.Hete
+
+open Unary prim val trm
+open ContextFreeGrammar
+
+namespace WeirdLogic
+
+def trm1 : trm := [lang| x := -x]
+def trm2 : trm := [lang| x := x + 1]
+def trm3 : trm := [lang| x := x * 2]
+def r1 : ContextFreeRule trm String :=
+  {
+    input := "L",
+    output := [Symbol.nonterminal "S1", Symbol.nonterminal "S2"],
+  }
+
+def r2 : ContextFreeRule trm String :=
+  {
+    input := "S1",
+    output := [Symbol.nonterminal "S3", Symbol.nonterminal "S1"],
+  }
+
+def r3 : ContextFreeRule trm String :=
+  {
+    input := "S1",
+    output := [],
+  }
+
+def r4 : ContextFreeRule trm String :=
+  {
+    input := "S2",
+    output := [Symbol.terminal trm1],
+  }
+
+def r5 : ContextFreeRule trm String :=
+  {
+    input := "S3",
+    output := [Symbol.terminal trm2],
+  }
+
+def r6 : ContextFreeRule trm String :=
+  {
+    input := "S3",
+    output := [Symbol.terminal trm3],
+  }
+
+def cfg1 : ContextFreeGrammar trm :=
+  {
+    NT := String,
+    initial := "S1",
+    rules := Finset.mk {r1, r2, r3, r4, r5, r6} (by unfold r1 r2 r3 r4 r5 r6 trm1 trm2 trm3; simp)
+  }
+
+def l1 : Language trm := cfg1.language
+
+lang_def prog_c1 :=
+  fun ⸨x: Val⸩ ⸨pa:Loc⸩ ⸨pb:Loc⸩ =>
+    let i := 0 in
+    let b := pb[i] in
+    while pb[i] {
+      let a := pa[i] in
+        if a > 0 then
+          x := x + 1
+        else
+          x := x*2;
+      i := i+1
+    };
+    x := -x
+
+abbrev multi_payload := List ℤ
+
+abbrev default_payload : multi_payload:= [0]
+abbrev default_trm : trm := [lang|()]
+
+def pay_idx_prod : Set (trm × multi_payload × multi_payload) :=
+  {
+    ([lang|()],(p,p)) | p ∈ @Set.univ multi_payload
+  }
+def lang_set : Set trm :=
+  {l | cfg1.Generates (expand_trm l) ∧ l ∈ @Set.univ trm}
+
+def lang_idx_prod : Set (trm × multi_payload × multi_payload ):=
+  { (l, ([0],[0])) | l ∈ lang_set}
+
+variable (pa_len : ℕ) (pb_len : ℕ) (xptr : loc)
+variable (paptr : trm × multi_payload × multi_payload -> loc) (pbptr : trm × multi_payload × multi_payload -> loc)
+
+lemma example4_spec' (f : ℤ -> val) (g q : ℤ -> val):
+  {
+    arr⟨⋆⟩(xptr , i in 1 =>f i) ∗
+    bighstar ⟪0,pay_idx_prod⟫ (fun i => harray i.val.2.1 (paptr i.val) ∗ harray i.val.2.2 (pbptr i.val))
+  }
+  [0| p in pay_idx_prod => prog_c1(⟨f 0⟩,⸨pa:Loc⸩, ⸨pb:Loc⸩)]
+  [1| l in lang_idx_prod => ⟦l.val.1⟧]
+  { v,
+    fun h => ∀ l ∈ lang_idx_prod, ∃ p ∈ pay_idx_prod , h ⟨1, l⟩ = h ⟨0, p⟩
+  }
+  := by
+  sorry
+
+/- Previously, constraints for payloads in the heap are in the post-condition
+    -- ∧ arr⟨{⟨0,p⟩}⟩(pa , i in pa_len => p.2.1[i]!) h
+    -- ∧ arr⟨{⟨0,p⟩}⟩(pb , i in pb_len => p.2.2[i]!) h
+  And pre-condition is default
+  -- arr⟨⋆⟩(pa , i in pa_len =>g i) ∗
+  -- arr⟨⋆⟩(pb , i in pb_len =>q i)
+-/
